qcp/ast/VC/alpha_equiv_proof_manual.v
@@ -240,11 +240,10 @@ Proof.
     rewrite H36, H39 in *; congruence.
   + destruct Hb as [Ha [x [Hx1 [Hx2 Hx3]]]].
     apply (alpha_equiv_quant_allvar qterm1_2 qterm2_2 qt1_2 qt2_2 qv1_2 qv2_2 str).
-    split; [auto | ].
-    rewrite H7 in H9.
-    rewrite H8 in H10.
-    split; [auto | ].
-    split; [auto | auto].
+    auto.
+    rewrite H7 in H9; auto.
+    rewrite H8 in H10; auto. 
+    auto.
 Qed.
 
 Lemma proof_of_alpha_equiv_return_wit_9_1 : alpha_equiv_return_wit_9_1.
